fairness/examples/ticketlock/group_roles.v
@@ -1,0 +1,147 @@
+From iris.proofmode Require Import tactics.
+From trillium.prelude Require Import finitary.
+
+(* TODO: move *)
+(* TODO: rename definitions inside? *)
+Section GroupRolesInstantiation.  
+  Context {Gl: Type} `{Countable Gl}.
+  Context (get_Gls: forall n, { gls: gset Gl | size gls = n}).
+  Let get_Gls' n := elements (proj1_sig (get_Gls n)). 
+
+  Instance Gl_inhabited: Inhabited Gl.
+  Proof. 
+    pose proof (get_Gls 1) as [gls SPEC].
+    destruct (decide (gls = ∅)).
+    { subst. set_solver. }
+    apply finitary.set_choose_L' in n as [g IN].
+    econstructor. apply g. 
+  Qed.
+
+  Let g0 := @inhabitant _ Gl_inhabited.
+
+  Definition gls' n: list Gl := 
+    let gls_Sn := get_Gls' (S n) in
+    if (decide (g0 ∈ gls_Sn)) 
+    then remove EqDecision0 g0 gls_Sn
+    else drop 1 gls_Sn. 
+      
+  Definition ρlg_i (n i: nat) := nth i (gls' n) g0.
+
+  (* TODO: move *)
+  Lemma nth_error_seq n i (DOM: i < n):
+    nth_error (seq 0 n) i = Some i.
+  Proof.
+    erewrite nth_error_nth' with (d := 0).
+    - f_equal. by apply seq_nth.
+    - by rewrite seq_length. 
+  Qed. 
+
+  (* TODO: move *)
+  Lemma length_remove_NoDup `{ED: EqDecision A} (l: list A) (a: A)
+                            (ND: NoDup l)
+    :
+    length (remove ED a l) = length l - (if (decide (a ∈ l)) then 1 else 0).
+  Proof.
+    destruct (decide (a ∈ l)) as [IN| ].
+    2: { rewrite notin_remove; [lia| ].
+         by intros ?%elem_of_list_In. }
+    apply elem_of_list_In, In_nth_error in IN as [i ITH].
+    pose proof ITH as (l1 & l2 & -> & LEN)%nth_error_split.
+    rewrite remove_app. rewrite notin_remove.
+    2: { apply NoDup_app in ND as (?&NIN&?).
+         intros IN1. apply (NIN a); [| set_solver]. by apply elem_of_list_In. }
+    simpl. rewrite decide_True; [| done].
+    rewrite notin_remove.
+    2: { rewrite cons_middle app_assoc in ND. 
+         apply NoDup_app in ND as (?&NIN&?).
+         intros ?%elem_of_list_In. apply (NIN a); set_solver. }
+    rewrite !app_length. simpl. lia.
+  Qed. 
+
+
+  Lemma get_Gls'_len n: length (get_Gls' n) = n. 
+  Proof.
+    rewrite /get_Gls'. 
+    destruct (get_Gls n) as [gls SPEC]; simpl in *.
+    rewrite -(list_to_set_elements_L gls) in SPEC.
+    rewrite size_list_to_set in SPEC; [lia| ].
+    apply NoDup_elements.
+  Qed. 
+
+  Lemma gls'_len n: length (gls' n) = n.
+  Proof. 
+    rewrite /gls'. destruct decide.
+    - rewrite length_remove_NoDup.
+      2: { rewrite /get_Gls'. apply NoDup_elements. }
+      rewrite decide_True; [| done].
+      rewrite get_Gls'_len. lia. 
+    - rewrite skipn_length.
+      rewrite get_Gls'_len. lia. 
+  Qed. 
+
+  Lemma gls'_ρlg n:
+    gls' n = map (ρlg_i n) (seq 0 n). 
+  Proof.
+    pose proof (gls'_len n) as LEN'. 
+    apply nth_ext with (d := g0) (d' := g0).
+    { by rewrite fmap_length seq_length. }
+
+    intros i DOM.    
+    eapply Some_inj.
+    rewrite -nth_error_nth'; [| done].
+    rewrite -nth_error_nth'. 
+    2: { rewrite fmap_length seq_length. congruence. }
+    rewrite nth_error_map.
+    rewrite nth_error_seq; [| congruence].
+    simpl. rewrite /ρlg_i.
+    by apply nth_error_nth'.
+  Qed.
+
+  Definition gls n: gset Gl := list_to_set (gls' n). 
+
+  Lemma gls_ρlg n:
+    gls n = list_to_set (map (ρlg_i n) (seq 0 n)).
+  Proof. 
+    rewrite /gls. f_equal. apply gls'_ρlg.
+  Qed. 
+
+  Lemma get_Gls'_NoDup n: NoDup (get_Gls' n).
+  Proof. 
+    rewrite /get_Gls'. apply NoDup_elements.
+  Qed.
+
+  (* TODO: move *)
+  Lemma NoDup_remove {A: Type} (l: list A)
+    (ND: NoDup l):
+    forall a EQ, NoDup (remove EQ a l).
+  Proof. 
+    intros a ?. revert a. induction l.
+    { done. }
+    intros. simpl. destruct EQ.
+    { subst. apply IHl. by inversion ND. }
+    econstructor.
+    2: { apply IHl. by inversion ND. }
+    inversion ND. subst.
+    intros IN%elem_of_list_In%in_remove.
+    apply H2. apply elem_of_list_In, IN. 
+  Qed. 
+
+  Lemma gls'_NoDup n: NoDup (gls' n).
+  Proof. 
+    rewrite /gls'. destruct decide.
+    - apply NoDup_remove. apply get_Gls'_NoDup.
+    - apply NoDup_ListNoDup.
+      eapply NoDup_app_remove_l.
+      erewrite take_drop.
+      apply NoDup_ListNoDup. apply get_Gls'_NoDup.
+  Qed. 
+
+  Lemma ρlg_i_dom_inj n:
+    forall i j, i < n -> j < n -> ρlg_i n i = ρlg_i n j -> i = j. 
+  Proof.
+    rewrite /ρlg_i.
+    rewrite -{1 2}(gls'_len n). apply NoDup_nth.
+    apply NoDup_ListNoDup. apply gls'_NoDup. 
+  Qed.
+
+End GroupRolesInstantiation.
